updates

intermediate2/Zeta.Intermediate.Correctness.fst
@@ -1,2 +1,135 @@
 module Zeta.Intermediate.Correctness
 
+open Zeta.App
+open Zeta.AppSimulate
+open Zeta.Time
+open Zeta.HashCollision
+open Zeta.Generic.Global
+open Zeta.Generic.Interleave
+open Zeta.Generic.TSLog
+open Zeta.Generic.Blum
+open Zeta.High.Interleave
+open Zeta.Intermediate.Global
+open Zeta.Intermediate.Interleave
+open Zeta.Intermediate.TSLog
+
+module S = FStar.Seq
+module GG = Zeta.Generic.Global
+
+(*
+ * A bunch of properties we use in the induction step:
+ *    (a) the intermediate verifiers all satisfy the store invariant
+ *    (b) the intermediate and spec level verifiers states correspond to one-another (related)
+ *    (c) the spec level log is time sorted (b and c imply that the spec log has type its_log)
+ *    (d) the spec level log is evict-add-consistent
+ * TODO: rename this
+ *)
+#push-options "--fuel 0 --ifuel 1 --query_stats"
+
+let induction_props #vcfg (ils: its_log vcfg) =
+  let ilk = to_logk ils in
+  spec_rel ils /\
+  is_eac ilk
+
+#pop-options
+
+let induction_props_or_hash_collision #vcfg (ils: its_log vcfg) =
+  o:option (hash_collision vcfg.app) {Some? o \/ induction_props ils}
+
+#push-options "--fuel 0 --ifuel 1 --query_stats"
+
+let lemma_empty_implies_induction_props #vcfg (il: verifiable_log vcfg)
+  : Lemma (ensures (length il = 0 ==> induction_props il))
+  = if length il = 0 then (
+      lemma_empty_implies_spec_rel il;
+      empty_implies_eac (to_logk il)
+    )
+
+let induction_props_snoc
+  (#vcfg:_)
+  (epmax: epoch)
+  (il: its_log vcfg {aems_equal_upto epmax il})
+  (i: seq_index il {let il' = prefix il i in
+                    (clock il i).e <= epmax /\
+                    induction_props il'})
+  : induction_props_or_hash_collision (prefix il (i+1))
+  = admit()
+
+
+#pop-options
+
+#push-options "--fuel 0 --ifuel 1 --query_stats"
+
+let rec induction_props_or_hash_collision_prefix_aux
+  (#vcfg:_)
+  (epmax: epoch)
+  (itsl: its_log vcfg {aems_equal_upto epmax itsl})
+  (i: nat{let itsl_ep = prefix_within_epoch epmax itsl in
+        i <= S.length itsl_ep})
+  : Tot (induction_props_or_hash_collision (prefix itsl i))
+    (decreases i)
+  = let itsl' = prefix itsl i in
+    lemma_empty_implies_induction_props itsl';
+    if i = 0 then None
+    else (
+      let i' = i - 1 in
+      let o = induction_props_or_hash_collision_prefix_aux epmax itsl i' in
+
+      prefix_within_epoch_correct epmax itsl i';
+      assert((clock itsl i').e <= epmax);
+
+      if Some? o then o
+      else
+        induction_props_snoc epmax itsl i'
+    )
+
+#pop-options
+
+let induction_props_or_hash_collision_prefix_ep
+  (#vcfg:_)
+  (epmax: epoch)
+  (itsl: its_log vcfg {aems_equal_upto epmax itsl})
+  : (let itsl_ep = prefix_within_epoch epmax itsl in
+     induction_props_or_hash_collision itsl_ep)
+  = let itsl_ep = prefix_within_epoch epmax itsl in
+    induction_props_or_hash_collision_prefix_aux epmax itsl (S.length itsl_ep)
+
+#push-options "--fuel 0 --ifuel 1 --query_stats"
+
+let lemma_verifier_correct
+  (#vcfg:_)
+  (epmax: epoch)
+  (gl: ms_verifiable_log vcfg epmax {S.length gl = vcfg.thread_count /\
+                                     ~ (seq_consistent (app_fcrs_within_ep epmax gl))})
+  : hash_collision vcfg.app
+  = (* interleaving of gl ordered by time of each log entry *)
+    let itsl = create gl in
+    lemma_add_evict_set_identical_glog epmax itsl;
+    assert(aems_equal_upto epmax itsl);
+
+    (* prefix upto epoch epmax *)
+    let itsl_ep = prefix_within_epoch epmax itsl in
+
+    (* we either find a hash collision or prove itsl_ep has some nice properties *)
+    let hc_or_props = induction_props_or_hash_collision_prefix_ep epmax itsl in
+    if Some? hc_or_props then
+      Some?.v hc_or_props
+    else (
+      assert(induction_props itsl_ep);
+
+      (* this implies the the hi-level log is evict-add-consistent *)
+      let itslk_ep = to_logk itsl_ep in
+      assert(is_eac itslk_ep);
+
+      (* seq of seq of app fn calls and their results which we know are not seq consistent *)
+      let app_calls_ss = app_fcrs_within_ep epmax gl in
+      assert(~ (seq_consistent app_calls_ss));
+
+      lemma_fcrs_within_epoch epmax itsl;
+      assert(GG.app_fcrs (to_glog itsl_ep) = app_calls_ss);
+
+      assert(GG.app_fcrs (to_glog itsl_ep) = GG.app_fcrs (to_glog itslk_ep));
+      Zeta.High.SeqConsistent.lemma_eac_implies_appfn_calls_seq_consistent itslk_ep;
+
+      hash_collision_contra vcfg.app
+    )
