intermediate2/Zeta.Intermediate.Global.fsti
@@ -1,6 +1,7 @@
 module Zeta.Intermediate.Global
 
 open Zeta.SSeq
+open Zeta.Time
 open Zeta.Intermediate.Verifier
 open Zeta.Intermediate.Logs
 open Zeta.Generic.Global
@@ -9,6 +10,9 @@ module IT = Zeta.Intermediate.Thread
 
 let verifiable_log (vcfg:_)
   = Zeta.Generic.Global.verifiable_log (int_verifier_spec vcfg)
+
+let ms_verifiable_log (vcfg:_) (epmax: epoch)
+  = gl: verifiable_log vcfg {aems_equal_upto epmax gl}
 
 let to_logk_entry (#vcfg:_) (gl: verifiable_log vcfg) (i: sseq_index gl)
   : logK_entry vcfg.app
